\debug{\tinysidebar{power-series-6/answer.tex}}
As a rational function
\begin{align*}
f(x)
&= \sum_{n=0}^\infty \biggl( 1 + \frac{2^n}{3^n}  \biggr) x^n \\
&= \sum_{n=0}^\infty \left( x^n + \frac{2^n}{3^n}  x^n \right) \\
&= \sum_{n=0}^\infty x^n + \sum_{n=0}^\infty \frac{2^n}{3^n}  x^n  \\
&= \frac{1}{1 - x} + \sum_{n=0}^\infty \left( \frac{2}{3} x \right) ^n  \\
&= \frac{1}{1 - x} + \frac{1}{1 - 2x/3} \\
&= \frac{1}{1 - x} + \frac{3}{3 - 2x} \\
&= \frac{3 - 2x + 3(1 - x)}{(1 - x)(3 - 2x)} \\
&= \frac{6 - 5x}{3 - 5x + 2x^2} \\
\end{align*}
