\tinysidebar{\debug{exercises/{cfg12/question.tex}}}
Here's a grammar with two variables.
\[
G:
\begin{cases}
S \rightarrow E \\
E \rightarrow E + E \st E * E \st a
\end{cases}
\]
where $\{S, E\}$ is set of variables, $S$ is the start variable, and 
$\{+, *, a\}$ is the set of terminals.
Terminals are like $\Sigma$ in DFAs.
Here are some string derivations from this $G$:
\begin{mylist}
\item[(a)] $S \implies E \implies E + E \implies E + a \implies a + a$
\item[(b)] $S \implies E \implies E + E \implies a + E \implies a + a$
\item[(b)] $S \implies E \implies E + E \implies a + E \implies a + E + E
\implies a + a + E \implies a + a + a$
\end{mylist}
Can you derive $a + a * a$ in two different ways?
(i.e., choose different orderings of production rules and/or different
order of variables to replace.)
What about $a + a + a$?
