\tinysidebar{\debug{exercises/{char0/answer.tex}}}
(a) Let $b_n = r^n$ be a solution of the recurrence relation.
Then
\[
r^n = 4 r^{n-1} - 4 r^{n-2}
\]
Hence
\[
r^2 - 4 r + 4 = 0
\]
Therefore the characteristic equation of the recurrence relation
is
\[
x^2 - 4x + 4 = 0
\]
(b)
Using the quadratic equation formula,
the roots of the characteristic equation from (a) are
\[
r = \frac{4 \pm \sqrt{4^2 - 4 \cdot 1 \cdot 4}}{2} = 2, 2
\]
(c)
The general closed form for $b_n$ is
\[
b_n = C_1 2^n + C_2 n2^n
\]
(d) From $b_0 = 1, b_1 = 1$, we have
\begin{align*}
  1 &= b_0 = C_1 \\
  1 &= b_1 = 2C_1 + 2C_2 
\end{align*}
Hence $C_1 = 1, C_2 = -1/2$.
Therefore
\[
b_n = 2^n - \frac{1}{2} n2^n
\]
for $n \geq 0$.

(Check:
$2^0 - \displaystyle\frac{1}{2} 0\cdot 2^0  = 1 = b_0$,
$2^1 - \displaystyle\frac{1}{2} 1\cdot 2^1 = 1 = b_1$.
So $2^n - \displaystyle\frac{1}{2} n2^n$ matches the
two base cases.
For $n = 2$,
$2^2 - \displaystyle\frac{1}{2}  2 \cdot 2^2 = 0$ and
$b_2 = 4b_1 - 4b_0 = 4\cdot 1 - 4\cdot 1 = 0$.)
