\debug{\tinysidebar{power-series-7/answer.tex}}
As a rational function
\begin{align*}
&\sum_{n=0}^\infty \biggl( \frac{2^n + (-1)^n}{3^n}  \biggr) x^n \\
&= \sum_{n=0}^\infty \biggl( \frac{2^n}{3^n} + \frac{(-1)^n}{3^n}  \biggr) x^n \\
&= \sum_{n=0}^\infty \biggl( \frac{2^n}{3^n}x^n + \frac{(-1)^n}{3^n}x^n  \biggr) \\
&= \sum_{n=0}^\infty \frac{2^n}{3^n}x^n + \sum_{n=0}^\infty \frac{(-1)^n}{3^n}x^n \\
&= \sum_{n=0}^\infty \left(\frac{2}{3}x\right)^n
+ \sum_{n=0}^\infty \left(\frac{-1}{3}x \right)^n \\
&= \frac{1}{1 - 2x/3} + \frac{1}{1 - (-x/3)} \\
&= \frac{3}{3 - 2x} + \frac{3}{3  + x} \\
&= \frac{3(3 + x) + 3(3 - 2x)}{(3 - 2x)(3 + x)}  \\
&= \frac{18 - 3x}{9 - 3x - 2x^2}  \\
\end{align*}

Check:
The following program
\VerbatimInput[frame=single,fontsize=\footnotesize]{exercises/power-series-7/test0.py}
\VerbatimInput[frame=single,fontsize=\footnotesize]{exercises/power-series-7/test0.txt}
