%-*-latex-*-
Q5. This is a continuation of Q4.

Modify your program to handle negative coefficients as follows. 
Here's a test case
\begin{console}[commandchars=\\\{\}]
\userinput{0 1 1 0 1 -1}
(x + 1)(x - 1) = x^2 - 1
\end{console}
Note that for the second polynomial on the left, instead of printing
\verb!(x + -1)!
the program prints
\verb!(x - 1)!.
Likewise, the polynomial on the right, instead of printing
\verb!x^2 + -1!
the program prints
\verb!x^2 - 1!.

Make sure your code passes all tests in the previous question.

\resett
\nextt
\begin{console}[commandchars=\\\{\}]
\userinput{0 1 1 0 1 -1}
(x + 1)(x - 1) = x^2 - 1
\end{console}

\nextt
\begin{console}[commandchars=\\\{\}]
\userinput{0 1 -1 0 1 -1}
(x - 1)(x - 1) = x^2 - 2x + 1
\end{console}

\nextt
\begin{console}[commandchars=\\\{\}]
\userinput{0 1 -2 0 1 -3}
(x - 2)(x - 3) = x^2 - 5x + 6
\end{console}

\nextt
\begin{console}[commandchars=\\\{\}]
\userinput{1 -2 3 0 -1 0}
(x^2 - 2x + 3)(-x) = -x^3 + 2x^2 - 3x
\end{console}
