%-*-latex-*-
\section{Recursion with Floors - Induction}

Now I'm going to show that 
\[
T(n) A\leq n + B n \log_2 n + C(n - 1)
\]
in a different way: using mathematical induction.

For simplicity, I'll assume that $A = B = C = 1$.
However the technique works for any constants $A, B, C$.

Note that the recurrence relation relates $T(n)$ to $T(\floor{n/2}))$
and not $T(n - 1)$.
This implies straightaway that we should use the weak form 
of mathematical induction.
Let's look at the inductive case of induction first.
Assume that
\[
T(k) \leq k + k \log_2 k + (k - 1)
\]
holds for for $k \leq n$.
By definition
\[
T(n + 1) = 2 T(\floor{(n+1)/2}) + n + 1
\]
By our induction hypothesis
\[
T(\floor{(n+1)/2}) 
\leq 
\floor{(n+1)/2}
+ \floor{(n+1)/2} \log_2 \floor{(n+1)/2} 
+ \floor{(n+1)/2} - 1
\]
By the definition of $T(n)$,
\[
T(n + 1) = 2 T(\floor{(n+1)/2}) + n + 1
\]
Putting things together we have
\begin{align*}
T(n + 1) 
&= 2 T(\floor{(n+1)/2}) + n + 1 \\
&\leq 2 
   \left( 
\floor{(n+1)/2}
+ \floor{(n+1)/2} \log_2 \floor{(n+1)/2} 
+ \floor{(n+1)/2} - 1       
   \right)
   + n + 1 \\
&\leq 2 
   \left( 
   (n+1)/2
+ ((n+1)/2) \log_2 ((n+1)/2) 
+ (n+1)/2 - 1       
   \right)
   + n + 1 \\
&= \left( 
   (n+1)
+ (n+1) \log_2 ((n+1)/2) 
+ (n+1) - 2       
   \right)
   + n + 1 \\
&= \left( 
   (n+1)
+ (n+1) [\log_2 (n+1) - 1]
+ (n+1) - 2       
   \right)
   + n + 1 \\
&= \left( 
   (n+1)
+ [(n+1)\log_2 (n+1) - (n+1)]
+ (n+1) - 2       
   \right)
   + n + 1 \\
&= \left( 
   (n+1)
+ (n+1)\log_2 (n+1)
 - 2       
   \right)
   + n + 1 \\
&= (n+1)
+ (n+1)\log_2 (n+1)   
   + n - 1 \\
\end{align*}
(The last couple of steps are easy, but make sure you understand them.)

I have just shown that if 
\[
T(k) \leq k + k \log_2 k + (k - 1)
\]
for $k \leq n$, then
\[
T(n+1) \leq (n+1) + (n+1) \log_2 (n+1) + ((n+1) - 1)
\]

The only thing left is the base case.
Note that by definition $T(0) = 1$
and 
\[
0 + 0 \log_2 0 + (0 - 1) = ...
\]
Hey ... wait a minute ... $\log_2 0$ is not defined!!!
What's happening???
[Well if you had paid close attention to the graphs drawn earlier you  
would have noticed that the graph of $n + \log_2(n) + (n - 1)$
does not begin at $n = 0$, right?]

That's not a problem. 
Why?
Because instead of proving 
\[
T(n) \leq n + n \log_2 n + (n - 1) \text{ for $n = 0, 1, 2, ...$}
\]
we can just prove 
\[
T(n) \leq n + n \log_2 n + (n - 1) \text{ for $n = 1, 2, 3, ...$}
\]
i.e. starting at $1$ or even $42$.
And why is that OK?

Because the goal is to prove a big-O statement.
And big-O statements is something about an inequality for
\textit{large} values of $n$.
And \textit{large} can mean 
\lq\lq$n \geq 1$ or
\lq\lq$n \geq 42$.
Correct?

Let's see if $n = 1$ works:
First
\[
T(1) = 1
\]
by definition.
For $n = 1$, 
\[
n + n \log_2 n + (n - 1) = 1 + 1 \log_2 1 + (1 - 1) = 1 + 0 + 0 = 1
\]
In other words
\[
T(n) \leq n + n \log_2 n + (n - 1)
\]
for $n = 1$.
So we have found our base case.

Now I'm ready to statement and prove the following formally:

\newpage

\begin{eg}
Let $T(n)$ be defined by 
\[
T(n) = 
\begin{cases}
1                       & \text{if $n = 0, 1$} \\
2T(\floor{n/2}) + n + 1 & \text{otherwise}
\end{cases}
\]
Show that, for $n \geq 1$,
\[
T(n) \leq n + n \log_2(n) + (n - 1)
\]
\end{eg}

\textit{Solution.}
For $n \geq 1$, let $P(n)$ be the statement
\[
P(n): \,\,\, T(n) \leq n + n \log_2(n) + (n - 1)
\]
We will prove that $P(n)$ is true for $n \geq 1$ by mathematical 
induction. 
For simplicity, we define $g(n)$ to be
\[
g(n) = n + n \log_2(n) + (n - 1)
\]

First, we prove the base case.
By definition
\[
T(1) = 1
\]
and
\[
g(1) = 1 + 1 \log_2 1 + (1 - 1) = 1 + 0 + 0 = 1
\]
Hence
\[
T(1) \leq g(1)
\]

Next, we prove the inductive case.
Let $n \geq 1$.
Assume that 
\[
P(k): \,\,\, T(k) 
\leq 
k
+ k \log_2 k 
+ (k - 1) 
\]
is true for all $k \leq n$.
We will now prove that $P(n+1)$ is true.
By definition
\[
T(n + 1) = 2 T(\floor{(n+1)/2}) + n + 1 \tag{1}
\]
In order to use the inductive hypothesis, 
we need to show 
\[
\floor{(n+1)/2} \leq n
\]
To do that we consider two cases.
If $n$ is even, say $n = 2k$, then
\[
\floor{(n+1)/2} = \floor{(2k + 1)/2} = \floor{k + 1/2} = k \leq 2k = n
\]
If $n$ is odd, say $n = 2k + 1$, then
\[
\floor{(n+1)/2} = \floor{(2k + 2)/2} = \floor{k + 1} = k + 1 \leq 2k + 1 = n
\]
We have shown that 
\[
\floor{(n+1)/2} \leq n
\]

Now, by our induction hypothesis,
$P(\floor{(n+1)/2})$ is true, i.e.,
\[
T(\floor{(n+1)/2}) 
\leq 
\floor{(n+1)/2}
+ \floor{(n+1)/2} \log_2 \floor{(n+1)/2} 
+ \floor{(n+1)/2} - 1 \tag{2}
\]
holds.
From (1) and (2), we have
\begin{align*}
T(n + 1) 
&= 2 T(\floor{(n+1)/2}) + n + 1 \\
&\leq 2 
   \left( 
\floor{(n+1)/2}
+ \floor{(n+1)/2} \log_2 \floor{(n+1)/2} 
+ \floor{(n+1)/2} - 1       
   \right)
   + n + 1 \\
&\leq 2 
   \left( 
   (n+1)/2
+ ((n+1)/2) \log_2 ((n+1)/2) 
+ (n+1)/2 - 1       
   \right)
   + n + 1 \\
&= \left( 
   (n+1)
+ (n+1) \log_2 ((n+1)/2) 
+ (n+1) - 2       
   \right)
   + n + 1 \\
&= \left( 
   (n+1)
+ (n+1) [\log_2 (n+1) - \log_2 2]
+ (n+1) - 2       
   \right)
   + n + 1 \\
&= \left( 
   (n+1)
+ (n+1) [\log_2 (n+1) - 1]
+ (n+1) - 2       
   \right)
   + n + 1 \\
&= \left( 
   (n+1)
+ [(n+1)\log_2 (n+1) - (n+1)]
+ (n+1) - 2       
   \right)
   + n + 1 \\
&= \left( 
   (n+1)
+ (n+1)\log_2 (n+1)
 - 2       
   \right)
   + n + 1 \\
&= (n+1)
+ (n+1)\log_2 (n+1)   
   + ((n + 1) - 1)
\end{align*}
i.e., $P(n+1)$ holds.

By mathematical induction, $P(n)$ is true for $n \geq 1$.
Therefore
\[
T(n) \leq n + n \log_2(n) + (n-1)
\]
for $n \geq 1$.
\qed

[EXERCISES]
