\debug{\tinysidebar{power-series-0/answer.tex}}
\newcommand\sdfs{\left(\frac{2}{3}\right)} % random
\begin{align*}
&(1 + 3x^2 + 5x^4) \sum_{n = 1}^\infty \frac{2^n}{3^n}x^n \\
&= \sum_{n = 1}^\infty \sdfs^n x^n
+ 3x^2 \sum_{n = 1}^\infty \sdfs^n x^n
+ 5x^4 \sum_{n = 1}^\infty \sdfs^n x^n
\\
 &= \sum_{n = 1}^\infty \sdfs^n x^n
 + \sum_{n = 1}^\infty 3 \sdfs^n x^{n+2}
 + \sum_{n = 1}^\infty 5 \sdfs^n x^{n+4}
 \\
 &= \sum_{n = 1}^\infty \sdfs^n x^n
 + \sum_{p = 3}^\infty 3 \sdfs^{p-2} x^{p}
 + \sum_{q = 5}^\infty 5 \sdfs^{q-4} x^{q} \,\,\,\text{(let $p=n+2$, $q=n+4$)}
 \\
&= \sum_{n = 1}^\infty \sdfs^n x^n
+ \sum_{n = 3}^\infty 3 \sdfs^{n-2} x^{n}
+ \sum_{n = 5}^\infty 5 \sdfs^{n-4} x^{n} \,\,\,\text{(replace $p$ by $n$, $q$ by $n$)}
\\
&=
\sdfs^1 x^1 + \sdfs^2 x^2 + \sdfs^3 x^3 + \sdfs^4 x^4 + \sum_{n = 5}^\infty \sdfs^n x^n \\
&\hspace{3.6cm} + 3 \sdfs^{1} x^{3} + 3 \sdfs^{2} x^{4} + \sum_{n = 5}^\infty 3 \sdfs^{n-2} x^{n} \\
&\hspace{8.2cm} + \sum_{n = 5}^\infty 5 \sdfs^{n-4} x^{n}
\\
 &=
 \frac{2}{3} x
 + \frac{4}{9} x^2
 + \frac{62}{27}x^3
 + \frac{124}{81}x^4
 + \sum_{n = 5}^\infty
 \left(
 \sdfs^n
 + 3 \sdfs^{n-2}
 + 5 \sdfs^{n-4} 
 \right) x^n
 \\
 &=
 \frac{2}{3} x
 + \frac{4}{9} x^2
 + \frac{62}{27}x^3
 + \frac{124}{81}x^4
 + \sum_{n = 5}^\infty
 \left(
 \sdfs^4 + 3 \sdfs^2 + 5
 \right) \sdfs^{n-4} x^n
 \\
 &=
 \frac{2}{3} x + \frac{4}{9} x^2 + \frac{62}{27}x^3 + \frac{124}{81}x^4
 +\sum_{n = 5}^\infty
 \frac{529}{81}
 \sdfs^{n-4} x^n
\end{align*}
Therefore the coefficient of $x^n$ is
\[
\begin{cases}
 0 & \text{ if } n = 0 \\
 2/3 & \text{ if } n = 1 \\
 4/9 & \text{ if } n = 2 \\
 62/27 & \text{ if } n = 3 \\
 124/81 & \text{ if } n = 4 \\
\displaystyle\frac{529}{81}\sdfs^{n-4}  & \text{ if } n \geq 5 
\end{cases}
\]
\qed
