\debug{\tinysidebar{power-series-4/answer.tex}}
As a power series,
\begin{align*}
f(x)
&= \frac{a}{b - cx} \\
&= \frac{a}{b} \cdot \frac{1}{1 - cx/b} \\
&= \frac{a}{b} \sum_{n=0}^\infty \left( \frac{cx}{b} \right)^n \\
&= \frac{a}{b} \sum_{n=0}^\infty \left( \frac{c}{b} \right)^n x^n\\
&= \sum_{n=0}^\infty \frac{a}{b} \left( \frac{c}{b} \right)^n x^n\\
\end{align*}
The coefficient of $x^n$ is
\[
\frac{a}{b} \left( \frac{c}{b} \right)^n
\]
for $n \geq 0$.

(Check: To test the above, you give $a,b,c$ some values and then
write a program that test the rational function against the power series
for some values of $x$.
For instance if you substitute $a=b=c=1$, the above gives you
\[
\frac{1}{1 - 1x} = \sum_{n=0}^\infty \frac{1}{1}\left(\frac{1}{1}\right)^n x^n
= \sum_{n=0}^\infty x^n
\]
which you already know is true.
You can then try using $a=2, b=3, c=4$ and test if
\[
\frac{2}{3 - 4x}
= \sum_{n=0}^\infty \frac{2}{3} \left( \frac{4}{3} \right)^n x^n
\]
is true.)
\qed
