\debug{\tinysidebar{exercises/recurrence-to-closed-form-1/answer.tex}}
Let
\[
a(x) = \sum_{n=0}^\infty a_n x^n
\]
Then
\begin{align*}
a(x)
&= \sum_{n=0}^\infty a_n x^n \\
&= a_0 + a_1x + \sum_{n=2}^\infty a_n x^n \\
&= 3 + 5x + \sum_{n=2}^\infty (a_{n-1} + a_{n-2}) x^n \\
&= 3 + 5x + \sum_{n=2}^\infty a_{n-1}x^n + \sum_{n=0}^\infty a_{n-2} x^n \\
&= 3 + 5x + x\sum_{n=2}^\infty a_{n-1}x^{n-1} + x^2\sum_{n=2}^\infty a_{n-2} x^{n-2} \\
&= 3 + 5x + x\sum_{p=1}^\infty a_{p}x^{p} + x^2\sum_{q=0}^\infty a_{q} x^{q}
\,\,\,\text{(let $p = n-1$ and $q=n-2$)}
\\
&= 3 + 5x + x\left( \sum_{p=0}^\infty a_{p}x^{p} - a_0 \right) + x^2a(x)
\\
&= 3 + 5x + x\left( a(x) - 3 \right) + x^2 a(x)
\\
&= 3 + 5x + x a(x) - 3x + x^2 a(x)
\\
&= 3 + 2x + x a(x) + x^2 a(x)
\\
\THEREFORE (1 - x - x^2) a(x)
&= 3 + 2x
\\
\THEREFORE  a(x)
&= \frac{3 + 2x}{1 - x - x^2}
\\
&= \frac{-3 - 2x}{x^2 + x -1}
\end{align*}
The roots of $x^2 + x -1$ are
\[
\frac{1 \pm \sqrt{5}}{2}
\]
Let
\[
r_1 = \frac{-1 + \sqrt{5}}{2}, \,\,\,
r_2 = \frac{-1 - \sqrt{5}}{2}
\]
By the theory of partial fractions, let
\[
\frac{-3 - 2x}{x^2 + x -1}
=
\frac{-3 - 2x}{(x - r_1)(x - r_2)}
=
\frac{A}{x - r_1} + \frac{B}{x - r_2}
\]
where $A,B$ are constants.
Then
\[
-3 - 2x
=
A(x - r_2) + B(x - r_1)
\]
If $x = r_1$, we get
\begin{align*}
-3 - 2r_1
&= A(r_1 - r_2)
\\
\THEREFORE
A
&= \frac{-3 - 2r_1}{r_1 - r_2} \\
&= \frac{-3 - 2r_1}{\sqrt{5}} \\
&= \frac{(-3 - 2r_1)\sqrt{5}}{5}
\end{align*}
And if $x = r_2$, we get
\begin{align*}
-3 - 2r_2
&= B(r_2 - r_1)
\\
\THEREFORE
B
&= \frac{-3 - 2r_2}{r_2 - r_1} \\
&= \frac{3 + 2r_2}{\sqrt{5}} \\
&= \frac{(3 + 2r_2)\sqrt{5}}{5}
\end{align*}
Hence
\[
a(x) = \frac{A}{x - r_1} + \frac{B}{x - r_2}
\]
where
\begin{align*}
A &= \frac{(-3 - 2r_1)\sqrt{5}}{5} \\
B &= \frac{(3 + 2r_2)\sqrt{5}}{5} \\
r_1 &= \frac{-1 + \sqrt{5}}{2} \\
r_2 &= \frac{-1 - \sqrt{5}}{2}
\end{align*}
Let's check with a program:
\VerbatimInput[frame=single,fontsize=\small]{exercises/recurrence-to-closed-form-1/main0.py}
The output is
\VerbatimInput[frame=single,fontsize=\small]{exercises/recurrence-to-closed-form-1/main0.txt}

Now we compute the coefficient of $x^n$ from the
partial fractions:
\begin{align*}
a(x)
&= \frac{A}{x - r_1} + \frac{B}{x - r_2} \\
&= -\frac{A}{r_1 - x} - \frac{B}{r_2 - x} \\
&= -\frac{A}{r_1} \frac{1}{1 - x/r_1} - \frac{B}{r_2} \frac{1}{1 - x/r_2} \\
&= -\frac{A}{r_1}\sum_{n=0}^\infty \left( \frac{x}{r_1} \right)^n
   - \frac{B}{r_2}\sum_{n=0}^\infty \left( \frac{x}{r_2} \right)^n\\
&= -\frac{A}{r_1}\sum_{n=0}^\infty  \frac{1}{r_1^n} x^n
   - \frac{B}{r_2}\sum_{n=0}^\infty \frac{1}{r_2^n} x^n\\
&= \sum_{n=0}^\infty
   \left( -\frac{A}{r_1^{n+1}}
   - \frac{B}{r_2^{n+1}}
   \right) x^n\\   
\end{align*}
Hence
\[
a_n = -\frac{A}{r_1^{n+1}} - \frac{B}{r_2^{n+1}}
\]
Let's check with a program:
\VerbatimInput[frame=single,fontsize=\small]{exercises/recurrence-to-closed-form-1/main1.py}
The output is
\VerbatimInput[frame=single,fontsize=\small]{exercises/recurrence-to-closed-form-1/main1.txt}

Simplifying $a_n$, we get
\begin{align*}
a_n
&= -\frac{A}{r_1^{n+1}} - \frac{B}{r_2^{n+1}}
\\
&= -A\left(\frac{r_2}{r_1r_2}\right)^{n+1} - B\left(\frac{r_1}{r_1r_2} \right)^{n+1}
\\
&=
\frac{1}{(r_1r_2)^{n+1}}
\left(
-A r_2^{n+1}
-B r_1^{n+1}
\right)
\\
&=
\frac{1}{(-1)^{n+1}}
\left(
-\frac{(-3 - 2r_1)\sqrt{5}}{5} r_2^{n+1} 
-\frac{(3 + 2r_2)\sqrt{5}}{5} r_1^{n+1}
\right)
\\
&=
\frac{(-1)^{n+1}\sqrt{5}}{5}
\left(
(3 + 2r_1) r_2^{n+1} 
-(3 + 2r_2) r_1^{n+1}
\right)
\\
&=
\frac{(-1)^{n+1}\sqrt{5}}{5}
\left(
\left( 3 + 2 \frac{-1 + \sqrt{5}}{2} \right) r_2^{n+1} 
-
\left( 3 + 2 \frac{-1 - \sqrt{5}}{2} \right) r_1^{n+1}
\right)
\\
&=
\frac{(-1)^{n+1}\sqrt{5}}{5}
\left(
\left( 2 + \sqrt{5} \right) r_2^{n+1} 
-
\left( 2 - \sqrt{5} \right) r_1^{n+1}
\right)
\end{align*}
Let's check with a program:
\VerbatimInput[frame=single,fontsize=\small]{exercises/recurrence-to-closed-form-1/main2.py}
The output is
\VerbatimInput[frame=single,fontsize=\small]{exercises/recurrence-to-closed-form-1/main2.txt}
Hence
\begin{align*}
a_n
&=
\frac{(-1)^{n+1}\sqrt{5}}{5}
\left(
\left( 2 + \sqrt{5} \right) r_2^{n+1} 
-
\left( 2 - \sqrt{5} \right) r_1^{n+1}
\right)
\\
&=
\frac{(-1)^{n+1}\sqrt{5}}{5}
\left(
\left( 2 + \sqrt{5} \right) \left( \frac{-1 - \sqrt{5}}{2} \right)^{n+1} 
-
\left( 2 - \sqrt{5} \right) \left( \frac{-1 + \sqrt{5}}{2} \right)^{n+1}
\right)
\end{align*}
for $n \geq 0$.
\qed
