\section{Reversal Function}

\begin{defn}
Let $x$ be a string. The \defone{reversal} of $x$, denoted $x^R$,
is just the same string with the letters reversed. Formally:
\begin{itemize}
 \item If $|x|=0$, then $x^R = \epsilon^R = \epsilon$.
 \item If $|x|>0$, then $x = ay$ where $a \in \Sigma$ and $x^R =
 y^Ra$.
\end{itemize}
\end{defn}


\newpage
\begin{ex}
Let $x,y \in \Sigma^*$. Prove that $(xy)^R = y^Rx^R$. (Yes, I know
it's obvious, but you still have to prove it.) [Hint: Induction.]
\end{ex}

\newpage
Now that I'm done defining the reversal of a string, I can
define the reversal of a language.

\begin{defn}
Let $L$ is a language then the reversal of a language is
\[
L^R = \{x^R \mid x \in L \}
\]
\end{defn}

For instance if $L = \{\ep, a, ab, abaa, abaaa\}$, then
\[
L^R = \{ \ep, a, ba, aaba, aaaba \}
\]
