\sectionthree{Linear nonhomogeneous recurrence relations}
\begin{python0}
from solutions import *; clear() 
\end{python0}

The general linear non-homogeneous case looks like this:
\[
a_n = c_1 a_{n-1} + \cdots c_d a_{n-d} + f(n)
\]
where $f(n)$ is a nonzero function in $n$.
Here's one example:
\[
a_n = 2a_{n-1} + n
\]
and here's another:
\[
a_n = a_{n-1} + 3a_{n-2} + 2n^3 + 1
\]
and yet another:
\[
a_n = a_{n-1} + 3a_{n-2} + \lfloor n \log n \rfloor
\]

Let's consider the a degree 2 nonhomogeneous recurrence relation:
\[
a_n = c_1 a_{n-1} + c_2 a_{n-2} + f(n), \,\,\,\,\, n \geq 2
\]
Of course using our method of generating functions,
in order to compute a closed form for $a_n$, we do this:
We let $a(x) = \sum_{n=0}^\infty a_n x^n$.
From 
\[
a_n = c_1 a_{n-1} + c_2 a_{n-2} + f(n), \,\,\,\,\, n \geq 2
\]
we get
\begin{align*}
a(x)
&= \sum_{n=0}^\infty a_n x^n \\
&= a_0 + a_1x + \sum_{n=0}^\infty a_n x^n \\
&= a_0 + a_1x + \sum_{n=2}^\infty (c_1 a_{n-1} + c_2 a_{n-2} + f(n))x^n \\
&= a_0 + a_1x + \sum_{n=2}^\infty (c_1 a_{n-1} + c_2 a_{n-2})x^n + 
\sum_{n=2}^\infty f(n)x^n \\
\end{align*}
Without going into details, we know that had the recurrence been this:
\[
a_n = c_1 a_{n-1} + c_2 a_{n-2}, \,\,\,\,\, n \geq 2
\]
we would have a rational function:
\[
a(x) = \frac{P(x)}{Q(x)}
\]
With the nonhomogeneous factor $f(n)$ in the recurrence relation we
get this:
\[
a(x) = \frac{P(x) + \sum_{n=2}^\infty f(n)x^n}{Q(x)}
\]
Therefore as long as we can express
\[
\sum_{n=2}^\infty f(n)x^n
\]
as a rational function then there is hope of getting the coefficient 
of $x^n$ of the power series of $a(x)$.

Let's try an example:
\[
a_n = 2a_{n-1} + n
\]
for $n \geq 1$.
Of course we let $a(x) = \sum_{n=0}^\infty a_n x^n$.
Then
\begin{align*}
a(x) 
&= \sum_{n=0} a_nx^n \\
&= a_0 + \sum_{n = 1}^\infty a_n x^n \\
&= a_0 + \sum_{n = 1}^\infty (2a_{n-1} + n) x^n \\
&= a_0 + 2\sum_{n = 1}^\infty a_{n-1}x^n + \sum_{n=1}^\infty n x^n \\
&= a_0 + 2x\sum_{n = 1}^\infty a_{n-1}x^{n-1} + \sum_{n=0}^\infty n x^n \\
\end{align*}
Notice that I've secretly actually added $0x^0$.
Continuing the computation we have
\begin{align*}
a(x) 
&= a_0 + 2x\sum_{n = 0}^\infty a_{n}x^{n} + \sum_{n=0}^\infty n x^n \\
&= a_0 + 2x a(x) + \sum_{n=0}^\infty n x^n \\
\therefore\,\,\,\,\, (1-2x) a(x) 
&= a_0 + \sum_{n=0}^\infty n x^n \\
\therefore\,\,\,\,\, a(x) 
&= \frac{a_0 + \sum_{n=0}^\infty n x^n}{1-2x} \\
\end{align*}
And by the way ... we can rewrite $\sum_{n=0}^\infty nx^n$ as a
rational function! It's just
\[
x\frac{d}{dx} \sum_{n=0}^\infty x^n
\]
remember?
Since
\begin{align*}
x\frac{d}{dx} \sum_{n=0}^\infty x^n
&= x \frac{d}{dx}\frac{1}{1-x} \\
x\frac{d}{dx} \sum_{n=0}^\infty x^n
&= x \frac{d}{dx} \frac{1}{1-x} \\
&= x \frac{1}{(1-x)^2} \\
\end{align*}
Hence
\begin{align*}
a(x) 
&= \frac{a_0 + \sum_{n=0}^\infty n x^n}{1-2x} \\
&= \frac{a_0 + \frac{x}{(1-x)^2}}{1-2x} \\
&= \frac{a_0(1-x)^2 + x}{(1-2x)(1-x)^2} \\
\end{align*}
Now we use the theory of partial fractions:
There are constants $A, B, C$ such that
\[
\frac{1}{(1-2x)(1-x)^2}
= 
\frac{A}{1-2x}
+
\frac{B}{1-x}
+
\frac{C}{(1-x)^2}
\]
We have
\[
1
= 
A(1-x)^2
+
B(1-x)(1-2x)
+
C(1-2x)
\]
When $x = 1$, we get $C = -1$.
When $x = 1/2$, we obtain $A = 4$.
Finally when $x = 0$, $1 = A + B + C$, and hence
$B = 1 - 4 + 1 = -2$.
Hence
\[
\frac{1}{(1-2x)(1-x)^2}
= 
\frac{4}{1-2x}
+
\frac{-2}{1-x}
+
\frac{-1}{(1-x)^2}
\]
Hence
\begin{align*}
a(x) 
&= 
(a_0(1-x)^2 + x) 
\biggl(
\frac{4}{1-2x}
+
\frac{-2}{1-x}
+
\frac{-1}{(1-x)^2}
\biggr) \\
&= 
(a_0 + (1-2a_0)x + a_0 x^2) 
\biggl(
4 \sum_{n=0}^\infty 2^n x^n
-2 \sum_{n=0}^\infty x^n
- \sum_{n=0}^\infty (n+1) x^n
\biggr) \\
&= 
(a_0 + (1-2a_0)x + a_0 x^2) 
\sum_{n=0}^\infty (4 \cdot 2^n - 2 - (n+1))x^n
\end{align*}
Hence 
\[
a_n = 
\begin{cases}
a_0 &\text{ if } n = 0 \\
%
a_0(4 \cdot 2 - 2 - (1+1)) + (1-2a_0)(4 - 2 - (0+1)) &\text{ if } n = 1 \\
%
a_0(4 \cdot 2^n - 2 - (n+1)) + (1-2a_0)(4 \cdot 2^{n-1} - 2 - n) +
a_0(4 \cdot 2^{n-2} - 2 - (n-1))
& \text{ if } n \geq 2 \\
\end{cases}
\]
Simplifying the above horrendous closed forms we get:
\[
a_n = 
\begin{cases}
a_0 &\text{ if } n = 0 \\
%
1 + 2a_0 &\text{ if } n = 1 \\
%
(2 + a_0)2^n - n  -2 & \text{ if } n \geq 2 \\
\end{cases}
\]

Let's check that the first few terms are correct.
First of all, $a_n = a_0$ for $n = 0$.
That's good.
For $n = 1$, from the closed form we have $a_1 = 1 + 2a_0$.
Now the recurrence we started with is
\[
a_n = 2a_{n-1} + n
\]
Therefore from the recurrence relation, $a_1 = 2a_0 + 1$.
That's also good.
One last check: Let's look at $n = 2$.
From the recurrence relation we have
\begin{align*}
a_2 &= 2a_1 + 2 \\
a_1 &= 2a_0 + 1
\end{align*}
Hence
\begin{align*}
a_2 = 2(2a_0 + 1) + 2 = 4a_0 + 4
\end{align*}
From the derived closed form we have
\[
(2 + a_0)2^2 - 2 - 2 = 8 + 4a_0 - 4 = 4a_0 + 4
\]



\input{exercises/non-homo0/main.tex}

\input{exercises/non-homo1/main.tex}
