\subsection{Tower of Hanoi}

Can the above method be used for a degree one recurrence relation?
Remember the Tower of Hanoi problem?
Let $t_n$ be the number of steps to solve the problem.
Recall that we solve the problem by providing
a recursive procedure.
Here's the problem again.
You have $n$ disks that you want to move from A to C.

\input{stdout02.tex}

We think of the $n$-disk problem in terms of the
$n-1$ disk problem:

\input{stdout03.tex}

We ignore disk $n$ for the time being
and apply our procedure to move the top $n-1$ disks from A to B:

\input{stdout04.tex}

This should take $t_{n-1}$ steps.
Now we move disk $n$ from A to C:

\input{stdout05.tex}

That takes 1 step.
And finally we apply our procedure to move
the $n-1$ disks from $B$ to $C$:

\input{stdout06.tex}

That takes $t_{n-1}$ steps.
Altogther we took $t_{n-1} + 1 + t_{n-1}$ steps.
Hence
\begin{align*}
t_n 
&= t_{n-1} + 1 + t_{n-1} \\
&= 2 t_{n-1} + 1
\end{align*}
We need a base condition.
So what's $t_0$?
That's the problem with $0$ disks.
It should probably be 0 step: $t_0 = 0$.
But vacuous problems are sometimes dangeourous.
So let's consider $t_1$.
Clearly $t_1 = 1$.
Now since we want $t_1 = 2t_0 + 1$, we have
\[
1 = 2 t_0 + 1
\]
and, yes, we do get $t_0 = 0$.
Altogether we have
\[
t_n = 
\begin{cases}
0 &\text{ if } n = 0 \\
2 t_{n-1} + 1 &\text{ if } n > 0
\end{cases}
\]
Furthermore note that the recurrence relation is not just defined
in terms of a linear combination of $t_n$'s for small $n$:
There's a \lq\lq + 1'' in the recurrence relation:
\[
t_n = 2 t_{n-1} \underline{ + 1 }
\]
This is a degree 1 nonhomogeneous recurrence relation.

For this recurrence relation, it's so simple that you can
actually find a closed form quickly, using \lq\lq substitutions".
Here's how you would do it.
\begin{align*}
t_n
&= 2 t_{n-1} + 1 \\ 
&= 2 ( 2t_{n-2} + 1) + 1 = 4t_{n-2} + 2 + 1 \\ 
&= 4 (2 t_{n-3} + 1 ) + 2 + 1 = 8 t_{n-3} + 4 + 2 + 1
\end{align*}
All the above assume that $n \geq 3$.
At this point you see a pattern:
\begin{align*}
t_n
&= 2^3 t_{n-3} + 2^2 + 2^1 + 2^0
\end{align*}
To check on the pattern, you do one more step (assuming $n \geq 4$):
\begin{align*}
t_n
&= 2^3 t_{n-3} + 2^2 + 2^1 + 2^0 \\ 
&= 2^3 (2t_{n-4} + 1) + 2^2 + 2^1 + 2^0 = 2^4t_{n-4} + 2^3 + 2^2 + 2^1 + 2^0
\end{align*}
i.e.,
\begin{align*}
t_n
&= 2^3 t_{n-3} + 2^2 + 2^1 + 2^0 \\ 
&= 2^4t_{n-4} + 2^3 + 2^2 + 2^1 + 2^0 \\
&= ... \\
&= 2^kt_{n-k} + 2^{k-1} + 2^{k-2} + \cdots + 2^3 + 2^2 + 2^1 + 2^0
\end{align*}
At some point you'd reach the base case, i.e., when $n - k = 1$,
\begin{align*}
t_n
&= 2^{n-1}t_{1} + 2^{n-2} + 2^{n-3} + \cdots + 2^3 + 2^2 + 2^1 + 2^0 \\
&= 2^{n-1} + 2^{n-2} + 2^{n-3} + \cdots + 2^3 + 2^2 + 2^1 + 2^0 \\
&= 2^n - 1
\end{align*}
by the geometric sum formula.
TADA!

So immediately, you know that to solve the tower of hanoi problem
you need to make $2^{32} - 1 = 4294967295$ move.

Now to be absolutely mathematically correct, the following
from the above:
\begin{align*}
t_n
&= 2^3 t_{n-3} + 2^2 + 2^1 + 2^0 \\ 
&= 2^4t_{n-4} + 2^3 + 2^2 + 2^1 + 2^0 \\
&= ... \\
&= 2^kt_{n-k} + 2^{k-1} + 2^{k-2} + \cdots + 2^3 + 2^2 + 2^1 + 2^0
\end{align*}
is not absolutely rigorous.
Why? Because it this:
\begin{align*}
t_n
&= ... (\leftarrow \text{look at the missing steps described by \lq\lq ..."}) \\ 
&= 2^kt_{n-k} + 2^{k-1} + 2^{k-2} + \cdots + 2^3 + 2^2 + 2^1 + 2^0
\end{align*}
The above leads to
\[
t_n = 2^n - 1
\]
Generally, this is what will happen in the mathematical derivation
of 
$t_n = 2^n - 1$.
The above is OK, as long as it is to derive a plausible closed form for $t_n$.
After that you prove $t_n = 2^n - 1$ is indeed true by induction, using the recurrence relation.

\input{exercises/tower0/main.tex}

\newpage
Another thing to note is this very importact fact:
\input{stdout07.tex}

\input{exercises/tower1/main.tex}

\newpage\myinput{tower-of-hanoi-variations.tex}

\input{exercises/tower2/main.tex}

\input{exercises/tower3/main.tex}

\input{exercises/tower4/main.tex}

\input{exercises/tower5/main.tex}

\input{exercises/tower6/main.tex}

\input{exercises/tower7/main.tex}

\myinput{tower-of-hanoi-generating-function.tex}
