\debug{\tinysidebar{exercises/recurrence-to-closed-form-0/answer.tex}}
Let
\[
b(x) = \sum_{n=0}^\infty b_n x^n
\]
Then
\begin{align*}
b(x)
&= \sum_{n=0}^\infty b_n x^n \\
&= b_0 + b_1x + \sum_{n=2}^\infty b_n x^n \\
&= 3 + 5x + \sum_{n=2}^\infty (7b_{n-1} + 11b_{n-2}) x^n \\
&= 3 + 5x + \sum_{n=2}^\infty 7b_{n-1}x^n + \sum_{n=0}^\infty 11b_{n-2} x^n \\
&= 3 + 5x + 7x\sum_{n=2}^\infty b_{n-1}x^{n-1}
+ 11x^2\sum_{n=2}^\infty b_{n-2} x^{n-2} \\
&= 3 + 5x + 7x\sum_{p=1}^\infty b_{p}x^{p}
+ 11x^2\sum_{q=0}^\infty b_{q} x^{q}
\,\,\,\text{(let $p = n-1$ and $q=n-2$)}
\\
&= 3 + 5x + 7x\left( \sum_{p=0}^\infty b_{p}x^{p} - b_0 \right)
+ 11x^2b(x)
\\
&= 3 + 5x + 7x\left( b(x) - 3 \right)
+ 11x^2b(x)
\\
&= 3 + 5x + 7x b(x) - 21x + 11x^2b(x)
\\
&= 3 -16x + 7x b(x) + 11x^2b(x)
\\
\THEREFORE (1 - 7x - 11x^2) b(x)
&= 3 -16x
\\
\THEREFORE  b(x)
&= \frac{3 - 16x}{1 - 7x - 11x^2}
\\
&= \frac{-3 + 16x}{11x^2 + 7x -1}
\end{align*}
The roots of $11x^2 + 7x -1$ are
\[
\frac{-7 \pm \sqrt{49 + 44}}{22}
=
\frac{-7 \pm \sqrt{93}}{22}
\]
Let
\[
r_1 = \frac{-7 + \sqrt{93}}{22}, \,\,\,
r_2 = \frac{-7 - \sqrt{93}}{22}
\]
By the theory of partial fractions, let
\[
\frac{-3 + 16x}{11x^2 + 7x -1}
=
\frac{-3 + 16x}{11(x - r_1)(x - r_2)}
=
\frac{A}{x - r_1} + \frac{B}{x - r_2}
\]
where $A,B$ are constants.
Then
\[
-3 + 16x
=
11A(x - r_2) + 11B(x - r_1)
\]
If $x = r_1$, we get
\begin{align*}
-3 + 16r_1
&= 11A(r_1 - r_2)
\\
\THEREFORE
A
&= \frac{-3 + 16r_1}{11(r_1 - r_2)} \\
&= \frac{-3 + 16r_1}{11(2\sqrt{93}/22)} \\
&= \frac{-3 + 16r_1}{\sqrt{93}} \\
&= \frac{(-3 + 16r_1)\sqrt{93}}{93} 
\end{align*}
And if $x = r_2$, we get
\begin{align*}
-3 + 16r_2
&= 11B(r_2 - r_1)
\\
\THEREFORE
B
&= \frac{-3 + 16r_2}{11(r_2 - r_1)} \\
&= \frac{-3 + 16r_2}{11(-2\sqrt{93}/22)} \\
&= \frac{3 - 16r_2}{\sqrt{93}} \\
&= \frac{(3 - 16r_2)\sqrt{93}}{93} 
\end{align*}
Hence
\[
b(x) = \frac{A}{x - r_1} + \frac{B}{x - r_2}
\]
where
\begin{align*}
A &= \frac{(-3 + 16r_1)\sqrt{93}}{93} \\
B &= \frac{(3 - 16r_2)\sqrt{93}}{93} \\
r_1 &= \frac{-7 + \sqrt{93}}{22} \\
r_2 &= \frac{-7 - \sqrt{93}}{22}
\end{align*}
Let's check with a program:
\VerbatimInput[frame=single,fontsize=\small]{exercises/recurrence-to-closed-form-0/main0.py}
The output is
\VerbatimInput[frame=single,fontsize=\small]{exercises/recurrence-to-closed-form-0/main0.txt}

Now we compute the coefficient of $x^n$ from the
partial fractions:
\begin{align*}
b(x)
&= \frac{A}{x - r_1} + \frac{B}{x - r_2} \\
&= -\frac{A}{r_1 - x} - \frac{B}{r_2 - x} \\
&= -\frac{A}{r_1} \frac{1}{1 - x/r_1} - \frac{B}{r_2} \frac{1}{1 - x/r_2} \\
&= -\frac{A}{r_1}\sum_{n=0}^\infty \left( \frac{x}{r_1} \right)^n
   - \frac{B}{r_2}\sum_{n=0}^\infty \left( \frac{x}{r_2} \right)^n\\
&= -\frac{A}{r_1}\sum_{n=0}^\infty  \frac{1}{r_1^n} x^n
   - \frac{B}{r_2}\sum_{n=0}^\infty \frac{1}{r_2^n} x^n\\
&= \sum_{n=0}^\infty
   \left( -\frac{A}{r_1^{n+1}}
   - \frac{B}{r_2^{n+1}}
   \right) x^n\\   
\end{align*}
Hence
\[
b_n = -\frac{A}{r_1^{n+1}} - \frac{B}{r_2^{n+1}}
\]
Let's check with a program:
\VerbatimInput[frame=single,fontsize=\small]{exercises/recurrence-to-closed-form-0/main1.py}
The output is
\VerbatimInput[frame=single,fontsize=\small]{exercises/recurrence-to-closed-form-0/main1.txt}

Simplifying $b_n$, we get
\begin{align*}
b_n
&= -\frac{A}{r_1^{n+1}} - \frac{B}{r_2^{n+1}}
\\
&= -A\left(\frac{r_2}{r_1r_2}\right)^{n+1} - B\left(\frac{r_1}{r_1r_2} \right)^{n+1}
\\
&=
\frac{1}{(r_1r_2)^{n+1}}
\left(
-A r_2^{n+1}
-B r_1^{n+1}
\right)
\\
&=
\frac{1}{(-44/22^2)^{n+1}}
\left(
-\frac{(-3 + 16r_1)\sqrt{93}}{93} r_2^{n+1} 
-\frac{(3 - 16r_2)\sqrt{93}}{93} r_1^{n+1}
\right)
\\
&=
(-1)^{n+1}
11^{n+1}
\left(
-\frac{(-3 + 16r_1)\sqrt{93}}{93} r_2^{n+1} 
-\frac{(3 - 16r_2)\sqrt{93}}{93} r_1^{n+1}
\right)
\\
&=
\frac{(-1)^{n+1}11^{n+1}\sqrt{93}}{93}
\left(
        \left( 3 - 16 r_1 \right) r_2^{n+1}
        +
        \left( -3 + 16 r_2 \right) r_1^{n+1}
\right)
\\
&=
\frac{(-1)^{n+1}11^{n+1}\sqrt{93}}{93}
\Biggl(
        \left( 3 - 16 \cdot \frac{-7 + \sqrt{93}}{22} \right)
        \left( \frac{-7 - \sqrt{93}}{22} \right)^{n+1}
        \\
&\hspace{3.7cm}        
        +
        \left( -3 + 16 \cdot \frac{-7 - \sqrt{93}}{22} \right)
        \left( \frac{-7 + \sqrt{93}}{22} \right)^{n+1}
\Biggr)
\\
&=
\frac{(-1)^{n+1}11^{n+1}\sqrt{93}}{93}
\Biggl(
        \left( 3 - 8 \cdot \frac{-7 + \sqrt{93}}{11} \right)
        \left( \frac{-7 - \sqrt{93}}{22} \right)^{n+1}
        \\
&\hspace{3.7cm}        
        +
        \left( -3 + 8 \cdot \frac{-7 - \sqrt{93}}{11} \right)
        \left( \frac{-7 + \sqrt{93}}{22} \right)^{n+1}
\Biggr)
\\
&=
\frac{(-1)^{n+1}11^{n+1}\sqrt{93}}{93}
\Biggl(
        \left( \frac{89 - 8\sqrt{93}}{11} \right)
        \left( \frac{-7 - \sqrt{93}}{22} \right)^{n+1}
        \\
&\hspace{3.7cm}        
        +
        \left( \frac{-89 - 8\sqrt{93}}{11} \right)
        \left( \frac{-7 + \sqrt{93}}{22} \right)^{n+1}
\Biggr)
\\
&=
\frac{(-1)^{n+1}11^{n}\sqrt{93}}{93}
\Biggl(
        \left( 89 - 8\sqrt{93} \right)
        \left( \frac{-7 - \sqrt{93}}{22} \right)^{n+1}
        \\
&\hspace{3.7cm}        
        +
        \left( -89 - 8\sqrt{93} \right)
        \left( \frac{-7 + \sqrt{93}}{22} \right)^{n+1}
\Biggr)
\\
\end{align*}
for $n \geq 0$.

Let's check with a program:
\VerbatimInput[frame=single,fontsize=\small]{exercises/recurrence-to-closed-form-0/main2.py}
The output is
\VerbatimInput[frame=single,fontsize=\small]{exercises/recurrence-to-closed-form-0/main2.txt}
