%-*-latex-*-
This is a continuation of Q2.

Modify the program so that instead of printing 
\verb!1x!, 
\verb!1x^2!, 
\verb!1x^3!, 
\verb!1x^4!, the program prints 
\verb!x!, \verb!x^2!, \verb!x^3!, \verb!x^4! 
(respectively). 
The following is a test case:
\begin{console}[commandchars=\\\{\}]
\userinput{0 1 1 0 1 1}
(x + 1)(x + 1) = x^2 + 2x + 1
\end{console}
Note that \verb!(x + 1)! is printed instead of  \verb!(1x + 1)!.

Make sure your code passes all the tests in the previous question.

\resett
\nextt
\begin{console}[commandchars=\\\{\}]
\userinput{0 1 1 0 1 1}
(x + 1)(x + 1) = x^2 + 2x + 1
\end{console}

\nextt
\begin{console}[commandchars=\\\{\}]
\userinput{0 1 1 0 1 -1}
(x + 1)(x + -1) = x^2 + -1
\end{console}

\nextt
\begin{console}[commandchars=\\\{\}]
\userinput{1 1 1 0 1 0}
(x^2 + x + 1)(x) = x^3 + x^2 + x
\end{console}

\nextt
\begin{console}[commandchars=\\\{\}]
\userinput{1 2 3 0 1 -1}
(x^2 + 2x + 3)(x + -1) = x^3 + x^2 + x + -3
\end{console}
