\tinysidebar{\debug{exercises/{non-linear17/answer.tex}}}
Let $n > n_0$.
Dividing the given recurrence by $g(n)$, we get
\[
  \frac{1}{g(n)} a_n = \frac{f(n)}{g(n)} + \sum_{i=0}^{n-1} h(i) a(i) \tag{1}
\]
We also have
\[
  \frac{1}{g(n-1)} a_{n-1} = \frac{f(n-1)}{g(n-1)} + \sum_{i=0}^{n-2} h(i) a(i) \tag{2}
\]
(1) $-$ (2) give us
\begin{align*}
  \frac{1}{g(n)} a_n - \frac{1}{g(n-1)} a_{n-1}
  &= \frac{f(n)}{g(n)} - \frac{f(n-1)}{g(n-1)} + h(n-1) a_{n-1} \\
  \THEREFORE
  \frac{1}{g(n)} a_n 
  &= \frac{f(n)}{g(n)} - \frac{f(n-1)}{g(n-1)} + h(n-1) a_{n-1} + \frac{1}{g(n-1)} a_{n-1}\\
  &= \frac{f(n)}{g(n)} - \frac{f(n-1)}{g(n-1)} + \left( h(n-1) + \frac{1}{g(n-1)} \right)
  a_{n-1}
  \\
  \THEREFORE
  a_n 
  &= f(n) - \frac{f(n-1)g(n)}{g(n-1)} + g(n)\left( h(n-1) + \frac{1}{g(n-1)} \right)
  a_{n-1}\\
\end{align*}
which is clearly a degree 1 recurrence.
