\debug{\tinysidebar{power-series-3/answer.tex}}
As a power series,
\begin{align*}
&1 + 2x + \frac{2}{3 + 4x} + \frac{5}{7x - 1}
\\
&=
1 + 2x +
\frac{2}{3} \cdot \frac{1}{1 - (-4x/3)}
-
5 \cdot \frac{1}{1 - 7x}
\\
&=
1 + 2x +
\frac{2}{3} \sum_{n=0}^\infty \left(\frac{-4x}{3}\right)^n
-
5 \cdot \sum_{n=0}^\infty (7x)^n
\\
&=
1 + 2x +
\frac{2}{3} \sum_{n=0}^\infty (-1)^n\left(\frac{4}{3}\right)^n x^n
-
5 \cdot \sum_{n=0}^\infty 7^nx^n
\\
&=
1 + 2x +
\sum_{n=0}^\infty (-1)^n\frac{2}{3}\left(\frac{4}{3}\right)^n x^n
-
\sum_{n=0}^\infty 5 \cdot 7^nx^n
\\
&=
1 + 2x +
\sum_{n=0}^\infty
\left(
(-1)^n\frac{2}{3}\left(\frac{4}{3}\right)^n
-
5 \cdot 7^n
\right)x^n
\\
 &=
 1 + 2x +
 \left((-1)^0\frac{2}{3} \cdot \left(\frac{4}{3}\right)^0 - 5 \cdot 7^0\right)
 +
 \left((-1)^1\frac{2}{3}\cdot \left(\frac{4}{3}\right)^1 - 5\cdot 7^1\right)x
 \\
 &\hspace{1.7cm} +
 \sum_{n=2}^\infty
 \left(
 (-1)^n\frac{2}{3} \left( \frac{4}{3} \right)^n
 -
 5 \cdot 7^n
 \right)x^n
 \\
 &=
 1 + 2x - \frac{13}{3} -\frac{323}{9} x
 +
 \sum_{n=2}^\infty
 \left(  
 (-1)^n \frac{2}{3} \left( \frac{4}{3} \right)^n
 -
 5 \cdot 7^n
 \right)x^n
 \\
 &=
 -\frac{10}{3} -\frac{305}{9} x
 +
 \sum_{n=2}^\infty
 \left(  
 (-1)^n\frac{2}{3} \left( \frac{4}{3} \right)^n
 -
 5 \cdot 7^n
 \right)x^n
\end{align*}
The coefficient of $x^n$ is
\[
\begin{cases}
-10/3 & \text{ if } n = 0 \\
-305/9 & \text{ if } n = 1 \\
\displaystyle (-1)^n \frac{2}{3} \left( \frac{4}{3} \right)^n
-
5 \cdot 7^n & \text{ if } n \geq 2 \\
\end{cases}
\]

Check:
The following program
\VerbatimInput[frame=single,fontsize=\footnotesize]{exercises/power-series-3/test0.py}
gives the following output:
\VerbatimInput[frame=single,fontsize=\footnotesize]{exercises/power-series-3/test0.txt}
\qed
